WIP: Progress on the termination proof of choose nat example

fairness/examples/choose_nat/choose_nat.v
@@ -16,16 +16,22 @@ Import derived_laws_later.bi.
 
 Set Default Proof Using "Type".
 
-Definition decr_loop_prog : val :=
-  rec: "go" "n" :=
-    if: "n" = #0 then #() else "go" ("n" - #1).
+Definition decr_loop_prog (l : loc) : val :=
+  rec: "go" <> :=
+    if: !#l = #0 then #() else #l <- (!#l - #1);; "go" #().
 
-Definition choose_nat_prog : val :=
+Definition choose_nat_prog (l : loc) : val :=
   λ: <>,
-     let: "n" := ChooseNat + #1 in
-     decr_loop_prog "n".
+     #l <- (ChooseNat + #1);;
+     decr_loop_prog l.
 
 Inductive CN := Start | N (n : nat).
+
+Definition F_CN (cn : CN) : Z :=
+  match cn with
+  | Start => -1
+  | N n => n
+  end.
 
 #[global] Instance CN_eqdec: EqDecision CN.
 Proof. solve_decision. Qed.
@@ -65,111 +71,248 @@ Defined.
 Definition the_model : LiveModel heap_lang the_cn_fair_model :=
   {| fuel_limit (x: fmstate the_cn_fair_model) := 40 %nat |}.
 
+Class choose_natPreG Σ := ChooseNatPreG {
+  choose_nat_G :> inG Σ (excl_authR ZO);
+ }.
+
+Class choose_natG Σ := ChooseNatG {
+  choose_nat_gname : gname;
+  choose_nat_preG :> inG Σ (excl_authR ZO);
+ }.
+
+Global Instance subG_choosenatΣ {Σ} :
+  subG (GFunctor (excl_authR ZO)) Σ → choose_natPreG Σ.
+Proof. solve_inG. Qed.
+
 Section proof.
-  Context `{!heapGS Σ the_cn_fair_model the_model}.
+  Context `{!heapGS Σ the_cn_fair_model the_model, choose_natG Σ}.
 
-  Lemma decr_loop_spec tid (n:nat) f :
+  Let Ns := nroot .@ "choose_nat".
+
+  Definition choose_nat_inv_inner (γ : gname) (l:loc) : iProp Σ :=
+    ∃ (cn:CN), frag_model_is cn ∗ l ↦ #(F_CN cn) ∗ own γ (●E (F_CN cn)).
+
+  Definition choose_nat_inv (γ : gname) (l:loc) :=
+    inv Ns (choose_nat_inv_inner γ l).
+
+  Lemma decr_loop_spec γ tid l (n:nat) f :
     6 ≤ f → f ≤ 40 →
-    {{{ has_fuel tid () f ∗ frag_free_roles_are ∅ ∗ frag_model_is (N (S n)) }}}
-      decr_loop_prog #(S n) @ tid
+    choose_nat_inv γ l -∗
+    {{{ has_fuel tid () f ∗ frag_free_roles_are ∅ ∗
+        own γ (◯E (Z.of_nat (S n))) }}}
+      decr_loop_prog l #() @ tid
     {{{ RET #(); tid ↦M ∅ }}}.
-  Proof.
-    iIntros (Hle1 Hle2 Φ) "(Hf & Hr & Hm) HΦ".
-    iInduction n as [|n] "IHn".
-    { wp_lam. wp_pures. wp_lam. wp_pures.
-      iApply (@wp_lift_pure_step_no_fork_singlerole_take_step
-              _ the_cn_fair_model _ _
-              (N 1) (N 0) tid _ _ (f - 6) (f - 3) _ _ _ _ ())=> /=;
-        [done|set_solver|lia|constructor|].
-      do 3 iModIntro.
-      rewrite has_fuel_fuels.
-      replace (f - 1 - 1 - 1 - 1 - 1 - 1) with (f - 6) by lia.
-      iFrame.
-      iIntros "Hm Hr Hf".
-      destruct (decide (() ∈ ∅)); [set_solver|].
-      wp_pures. by iApply "HΦ". }
-    wp_lam.
-    rewrite fmap_insert fmap_empty. (* Sigh.. *)
-    wp_pures.
-    rewrite fmap_insert fmap_empty. (* Sigh.. *)
-    wp_pures.
-    rewrite fmap_insert fmap_empty. (* Sigh.. *)
-    iApply (@wp_lift_pure_step_no_fork_singlerole_take_step
-              _ the_cn_fair_model _ _
-              (N $ S $ S n) (N $ S n) tid _ _ (f - 3) f _ _ _ _ ())=> /=;
-      [done|done|set_solver|lia|constructor|].
-    do 3 iModIntro.
-    rewrite has_fuel_fuels.
-    replace (f - 1 - 1 - 1) with (f - 3) by lia.
-    iFrame.    
-    iIntros "Hm Hr Hf".
-    wp_pures.
-    replace (Z.of_nat (S $ S n) - 1)%Z with (Z.of_nat $ S n) by lia.
-    destruct (decide (() ∈ {[()]})); [|set_solver].
-    rewrite has_fuel_fuels.
-    by iApply ("IHn" with "Hf Hr Hm").
-  Qed.
+  Proof. Admitted.
 
-  Lemma choose_nat_spec tid f :
+  (* Lemma decr_loop_spec γ tid l (n:nat) f : *)
+  (*   6 ≤ f → f ≤ 40 → *)
+  (*   {{{ has_fuel tid () f ∗ frag_free_roles_are ∅ ∗ *)
+  (*       own γ (◯E (Z.of_nat (S n))) }}} *)
+  (*     decr_loop_prog l @ tid *)
+  (*   {{{ RET #(); tid ↦M ∅ }}}. *)
+  (* Proof. *)
+  (*   iIntros (Hle1 Hle2 Φ) "(Hf & Hr & Hm) HΦ". *)
+  (*   iInduction n as [|n] "IHn". *)
+  (*   { wp_lam. wp_pures. wp_lam. wp_pures. *)
+  (*     iApply (@wp_lift_pure_step_no_fork_singlerole_take_step *)
+  (*             _ the_cn_fair_model _ _ *)
+  (*             (N 1) (N 0) tid _ _ (f - 6) (f - 3) _ _ _ _ ())=> /=; *)
+  (*       [done|set_solver|lia|constructor|]. *)
+  (*     do 3 iModIntro. *)
+  (*     rewrite has_fuel_fuels. *)
+  (*     replace (f - 1 - 1 - 1 - 1 - 1 - 1) with (f - 6) by lia. *)
+  (*     iFrame. *)
+  (*     iIntros "Hm Hr Hf". *)
+  (*     destruct (decide (() ∈ ∅)); [set_solver|]. *)
+  (*     wp_pures. by iApply "HΦ". } *)
+  (*   wp_lam. *)
+  (*   rewrite fmap_insert fmap_empty. (* Sigh.. *) *)
+  (*   wp_pures. *)
+  (*   rewrite fmap_insert fmap_empty. (* Sigh.. *) *)
+  (*   wp_pures. *)
+  (*   rewrite fmap_insert fmap_empty. (* Sigh.. *) *)
+  (*   iApply (@wp_lift_pure_step_no_fork_singlerole_take_step *)
+  (*             _ the_cn_fair_model _ _ *)
+  (*             (N $ S $ S n) (N $ S n) tid _ _ (f - 3) f _ _ _ _ ())=> /=; *)
+  (*     [done|done|set_solver|lia|constructor|]. *)
+  (*   do 3 iModIntro. *)
+  (*   rewrite has_fuel_fuels. *)
+  (*   replace (f - 1 - 1 - 1) with (f - 3) by lia. *)
+  (*   iFrame.     *)
+  (*   iIntros "Hm Hr Hf". *)
+  (*   wp_pures. *)
+  (*   replace (Z.of_nat (S $ S n) - 1)%Z with (Z.of_nat $ S n) by lia. *)
+  (*   destruct (decide (() ∈ {[()]})); [|set_solver]. *)
+  (*   rewrite has_fuel_fuels. *)
+  (*   by iApply ("IHn" with "Hf Hr Hm"). *)
+  (* Qed. *)
+
+  Lemma choose_nat_spec γ l tid f :
     8 ≤ f → f ≤ 40 →
-    {{{ has_fuel tid () f ∗ frag_free_roles_are ∅ ∗ frag_model_is Start }}}
-      choose_nat_prog #() @ tid
+    choose_nat_inv γ l -∗
+    {{{ has_fuel tid () f ∗ frag_free_roles_are ∅ ∗
+        own γ (◯E (-1)%Z) }}}
+      choose_nat_prog l #() @ tid
     {{{ RET #(); tid ↦M ∅ }}}.
-  Proof.
-    iIntros (Hle1 Hle2 Φ) "(Hf & Hr & Hm) HΦ".
-    wp_lam.
-    wp_bind ChooseNat.
-    iApply (wp_choose_nat_nostep _ _ _ {[() := (f - 2)]} with "[Hf]").
-    { set_solver. }
-    { rewrite -has_fuel_fuels_S has_fuel_fuels.
-      replace (S (f - 2)) with (f - 1) by lia. done. }
-    iIntros "!>" (n) "Hf".
-    iApply (@wp_lift_pure_step_no_fork_singlerole_take_step
-              _ the_cn_fair_model _ _
-              Start (N $ S n) tid _ _ (f - 2) f _ _ _ _ ())=> /=;
-      [done|done|set_solver|lia|constructor|].
-    do 3 iModIntro.
-    rewrite has_fuel_fuels.
-    iFrame.
-    iIntros "Hm Hr Hf".
-    destruct (decide (() ∈ {[()]})); [|set_solver].
-    wp_pures.
-    replace (Z.of_nat n + 1)%Z with (Z.of_nat $ S n) by lia.
-    rewrite -has_fuel_fuels.
-    iApply (decr_loop_spec with "[$Hm $Hr $Hf]"); [lia|lia|].
-    done.
-  Qed.
+  Proof. Admitted.
 
-End proof.    
+  (*   iIntros (Hle1 Hle2 Φ) "(Hf & Hr & Hm) HΦ". *)
+  (*   wp_lam. *)
+  (*   wp_bind ChooseNat. *)
+  (*   iApply (wp_choose_nat_nostep _ _ _ {[() := (f - 2)]} with "[Hf]"). *)
+  (*   { set_solver. } *)
+  (*   { rewrite -has_fuel_fuels_S has_fuel_fuels. *)
+  (*     replace (S (f - 2)) with (f - 1) by lia. done. } *)
+  (*   iIntros "!>" (n) "Hf". *)
+  (*   iApply (@wp_lift_pure_step_no_fork_singlerole_take_step *)
+  (*             _ the_cn_fair_model _ _ *)
+  (*             Start (N $ S n) tid _ _ (f - 2) f _ _ _ _ ())=> /=; *)
+  (*     [done|done|set_solver|lia|constructor|]. *)
+  (*   do 3 iModIntro. *)
+  (*   rewrite has_fuel_fuels. *)
+  (*   iFrame. *)
+  (*   iIntros "Hm Hr Hf". *)
+  (*   destruct (decide (() ∈ {[()]})); [|set_solver]. *)
+  (*   wp_pures. *)
+  (*   replace (Z.of_nat n + 1)%Z with (Z.of_nat $ S n) by lia. *)
+  (*   rewrite -has_fuel_fuels. *)
+  (*   iApply (decr_loop_spec with "[$Hm $Hr $Hf]"); [lia|lia|]. *)
+  (*   done. *)
+  (* Qed. *)
 
-#[local] Instance the_model_terminates :
-  FairTerminatingModel the_cn_fair_model.
-Proof. Admitted. 
+End proof.
+
+(* Theorem choose_nat_terminates *)
+(*         (extr : extrace) (Hvex : extrace_valid extr) *)
+(*         (Hexfirst : (trfirst extr).1 = [choose_nat_prog #()]): *)
+(*   (∀ tid, fair_ex tid extr) -> terminating_trace extr. *)
+(* Proof. *)
+
+Inductive the_order : CN → CN → Prop :=
+  | Start_order cn : the_order cn Start
+  | N_order n1 n2 : n1 ≤ n2 → the_order (N n1) (N n2).
+
+Local Instance the_order_po: PartialOrder the_order.
+Proof.
+  split.
+  - split.
+    + by intros []; constructor.
+    + intros [] [] [] Hc12 Hc23; try constructor.
+      * inversion Hc23.
+      * inversion Hc12.
+      * inversion Hc23.
+      * inversion Hc12. inversion Hc23. simplify_eq. lia.
+  - intros [] []; inversion 1; simplify_eq; try eauto; try inversion 1.
+    simplify_eq. f_equal. lia.
+Qed.
+
+Definition the_decreasing_role (s : fmstate the_cn_fair_model) : unit :=
+  match s with | _ => () end.
+
+#[local] Program Instance the_model_terminates :
+  FairTerminatingModel the_cn_fair_model :=
+  {|
+    ftm_leq := the_order;
+    ftm_decreasing_role := the_decreasing_role;
+  |}.
+Next Obligation.
+  assert (∀ n, Acc (strict the_order) (N n)).
+  { intros n.
+    induction n as [n IHn] using lt_wf_ind.
+    constructor. intros cn [Hcn1 Hcn2].
+    inversion Hcn1 as [|n1 n2]; simplify_eq.
+    destruct (decide (n = n1)) as [->|Hneq]; [done|].
+    apply IHn. lia. }
+  constructor. intros [] [Hc1 Hc2]; [|done].
+  inversion Hc1; simplify_eq. done.
+Qed.
+Next Obligation.
+  intros cn [ρ' [cn' Htrans]]. simpl in *.
+  split.
+  - rewrite /the_decreasing_role. simpl. rewrite /cn_live_roles.
+    destruct cn; [set_solver|].
+    destruct n; [inversion Htrans|set_solver].
+  - intros cn'' Htrans'.
+    destruct cn.
+    + split.
+      * constructor.
+      * intros Hrel. inversion Hrel; simplify_eq.
+        inversion Htrans'.
+    + split.
+      * destruct cn''.
+        -- inversion Htrans'.
+        -- inversion Htrans'; simplify_eq.
+           constructor. lia.
+      * intros Hrel.
+        inversion Htrans'; simplify_eq.
+        inversion Hrel; simplify_eq.
+        lia.
+Qed.
+Next Obligation. done. Qed.
+Next Obligation.
+  intros cn1 ρ cn2 Htrans.
+  destruct cn1.
+  - inversion Htrans; simplify_eq. constructor.
+  - inversion Htrans; simplify_eq. constructor. lia.
+Qed.
 
 #[local] Instance proof_irrel_trans s x :
   ProofIrrel ((let '(s', ℓ) := x in cntrans s ℓ s'): Prop).
 Proof. apply make_proof_irrel. Qed.
 
-Lemma model_finitary s :
-  Finite { '(s', ℓ) | cntrans s ℓ s'}.
+Definition ξ_cn (l:loc) (extr : execution_trace heap_lang)
+           (auxtr : finite_trace the_cn_fair_model (option unit)) :=
+  ∃ (cn:CN), (trace_last extr).2.(heap) !! l = Some #(F_CN cn) ∧
+             (trace_last auxtr) = cn.
+
+#[local] Instance proof_irrel_ξ l oζ c' ex atr ℓ δ' :
+  ProofIrrel (sim_rel_with_user the_cn_fair_model the_model
+                  (ξ_cn l) (ex :tr[ oζ ]: c') (atr :tr[ ℓ ]: δ')).
+Proof. apply make_proof_irrel. Qed.
+
+#[local] Instance eq_decision_the_model :
+  EqDecision (live_model_to_model the_cn_fair_model the_model).
 Proof. Admitted.
 
-Theorem choose_nat_terminates
+#[local] Instance eq_decision_mlabel :
+  EqDecision (mlabel (live_model_to_model the_cn_fair_model the_model)).
+Proof. solve_decision. Qed.
+
+Theorem choose_nat_sim l
         (extr : extrace) (Hvex : extrace_valid extr)
-        (Hexfirst : (trfirst extr).1 = [choose_nat_prog #()]):
-  (∀ tid, fair_ex tid extr) -> terminating_trace extr.
+        (Hexfirst : (trfirst extr).1 = [choose_nat_prog l #()]):
+  continued_simulation (sim_rel_with_user the_cn_fair_model the_model (ξ_cn l)) (trace_singleton ([choose_nat_prog l #()], {| heap := <[l:=#-1]>∅; used_proph_id := ∅ |}))
+                       (trace_singleton (initial_ls (LM := the_model) Start 0%nat)).
 Proof.
-  eapply (simulation_adequacy_terminate_ftm (Mdl := the_cn_fair_model) (heapΣ the_cn_fair_model) NotStuck _ Start ∅) =>//.
-  { eapply valid_state_evolution_finitary_fairness.
-    intros ?. simpl. apply (model_finitary s1). }
-  iIntros (HGS) "!> Hm Hr Hs !>".
-  simpl.
-  replace (∅ ∖ {[()]}) with (∅:gset unit) by set_solver.
-  rewrite -fmap_gset_to_gmap.
-  rewrite /gset_to_gmap. simpl.
-  repeat rewrite fmap_insert.
-  repeat rewrite fmap_empty.
-  rewrite -has_fuel_fuels.
-  iApply (choose_nat_spec with "[$Hm $Hr $Hs]"); [simpl;lia|simpl;lia|].
-  eauto.
-Qed.
+  assert (heapGpreS #[GFunctor (excl_authR ZO); heapΣ the_cn_fair_model] the_cn_fair_model the_model) as HPreG.
+  { apply _. }
+  eapply (strong_simulation_adequacy).
+  { done. }
+  { clear.
+    intros extr atr c' oζ.
+    eapply finite_smaller_card_nat.
+    simpl.
+    eapply (in_list_finite [(_,_)]).
+    intros [δ' ℓ] [Hrel [cn [Hextr Hatr]]].
+    admit. }
+Admitted.
+
+(* Theorem choose_nat_terminates l *)
+(*         (extr : extrace) (Hvex : extrace_valid extr) *)
+(*         (Hexfirst : (trfirst extr).1 = [choose_nat_prog l #()]): *)
+(*   (∀ tid, fair_ex tid extr) -> terminating_trace extr. *)
+(* Proof. *)
+(*   eapply (simulation_adequacy_terminate_ftm (Mdl := the_cn_fair_model) (heapΣ the_cn_fair_model) NotStuck _ Start ∅) =>//. *)
+(*   { eapply valid_state_evolution_finitary_fairness. *)
+(*     intros ?. simpl. apply (model_finitary s1). } *)
+(*   iIntros (HGS) "!> Hm Hr Hs !>". *)
+(*   simpl. *)
+(*   replace (∅ ∖ {[()]}) with (∅:gset unit) by set_solver. *)
+(*   rewrite -fmap_gset_to_gmap. *)
+(*   rewrite /gset_to_gmap. simpl. *)
+(*   repeat rewrite fmap_insert. *)
+(*   repeat rewrite fmap_empty. *)
+(*   rewrite -has_fuel_fuels. *)
+(*   iApply (choose_nat_spec with "[$Hm $Hr $Hs]"); [simpl;lia|simpl;lia|]. *)
+(*   eauto. *)
+(* Qed. *)
